Construct $\ket{\dotprod{\physvec{S}}{\physvec{\hat{n}}}; \plus}$ such that
\[
\dotprod{\physvec{S}}{\physvec{\hat{n}}}
\ket{\dotprod{\physvec{S}}{\physvec{\hat{n}}}; \plus}
=
\left(\frac{\hbar}{2}\right)
\ket{\dotprod{\physvec{S}}{\physvec{\hat{n}}}; \plus}
\]
where $\physvec{\hat{n}}$ is characterized by a polar angle $\beta$ and
azimuthal angle $\alpha$.  Express your answer as a linear combination
of $\ket{\plus}$ and $\ket{\minus}$

\subsection*{Solution}

Stating $\physvec{\hat{n}}$ in terms of the cartesian projection for
spherical coordinates gives us $[ \sin\beta\cos\alpha,
  \sin\beta\sin\alpha, \cos\beta ]$.  If we take $\physvec{S} = [S_x,
  S_y, S_z]$, then we get
\[
\dotprod{\physvec{S}}{\physvec{\hat{n}}} =
\sin\beta\cos\alpha S_x
+\sin\beta\sin\alpha S_y
+\cos\beta S_z
\]
Now take the values of $S_x$, $S_y$, and $S_z$:
\begin{align*}
  S_x &= \frac{\hbar}{2}(\outerprod{\plus}{\minus} + \outerprod{\minus}{\plus}) \\
  S_y &= \frac{i\hbar}{2}(\outerprod{\minus}{\plus} - \outerprod{\plus}{\minus}) \\
  S_z &= \frac{\hbar}{2}(\outerprod{\plus}{\plus} - \outerprod{\minus}{\minus})
\end{align*}
Now combine the two:
\begin{align*}
  \dotprod{\physvec{S}}{\physvec{\hat{n}}}
  &=
  \frac{\hbar}{2}\sin\beta\cos\alpha\outerprod{\plus}{\minus}
  +\frac{\hbar}{2}\sin\beta\cos\alpha\outerprod{\minus}{\plus} \\
  &+\frac{i\hbar}{2}\sin\beta\sin\alpha\outerprod{\minus}{\plus}
  -\frac{i\hbar}{2}\sin\beta\sin\alpha\outerprod{\plus}{\minus} \\
  &+\frac{\hbar}{2}\cos\beta\outerprod{\plus}{\plus}
  -\frac{\hbar}{2}\cos\beta\outerprod{\minus}{\minus} \\
  &=
  \frac{\hbar}{2}\sin\beta(\cos\alpha + i\sin\alpha)\outerprod{\plus}{\minus}
  +\frac{\hbar}{2}\sin\beta(\cos\alpha - i\sin\alpha)\outerprod{\minus}{\plus} \\
  &+ \frac{\hbar}{2}\cos\beta\outerprod{\plus}{\plus}
  -\frac{\hbar}{2}\cos\beta\outerprod{\minus}{\minus} \\
  &=
  \frac{\hbar}{2}\cos\beta\outerprod{\plus}{\plus}
  -\frac{\hbar}{2}\cos\beta\outerprod{\minus}{\minus}
  +\frac{\hbar}{2}e^{i\alpha}\sin\beta\outerprod{\plus}{\minus}
  +\frac{\hbar}{2}e^{-i\alpha}\sin\beta\outerprod{\minus}{\plus}
\end{align*}
The matrix form of this is
\[
\frac{\hbar}{2}
\begin{bmatrix}
  \cos\beta & e^{-i\alpha}\sin\beta \\
  e^{i\alpha}\sin\beta & -\cos\beta \\
\end{bmatrix}
\]
Now find the eigenvalues:
\[
\left|
\begin{bmatrix}
  \frac{\hbar}{2}\cos\beta - \lambda & \frac{\hbar}{2}e^{-i\alpha}\sin\beta \\
  \frac{\hbar}{2}e^{i\alpha}\sin\beta & -\frac{\hbar}{2}\cos\beta - \lambda \\
\end{bmatrix}
\right|
= 0
\]
This gives us:
\begin{align*}
  \left(\frac{\hbar}{2}\cos\beta - \lambda\right)
  \left(-\frac{\hbar}{2}\cos\beta - \lambda\right)
  -\frac{\hbar}{2}e^{i\alpha}\sin\beta
  \frac{\hbar}{2}e^{-i\alpha}\sin\beta &= 0 \\
  \left(\frac{\hbar}{2}\cos\beta - \lambda\right)
  \left(\frac{\hbar}{2}\cos\beta + \lambda\right)
  +\frac{\hbar^2}{4}\sin^2\beta &= 0 \\
  \frac{\hbar^2}{4}\cos^2\beta + \frac{\hbar^2}{4}\sin^2\beta &= \lambda^2 \\
  \frac{\hbar^2}{4}(\cos^2\beta + \sin^2\beta) &= \lambda^2 \\
  \pm\frac{\hbar}{2} &= \lambda \\
\end{align*}

Now find the eigenvectors by solving
\[
\begin{bmatrix}
  \frac{\hbar}{2}\cos\beta - \lambda & \frac{\hbar}{2}e^{-i\alpha}\sin\beta \\
  \frac{\hbar}{2}e^{i\alpha}\sin\beta & -\frac{\hbar}{2}\cos\beta - \lambda \\
\end{bmatrix}
\begin{bmatrix}
  k_{\plus} \\
  k_{\minus}
\end{bmatrix}
=
\pm\frac{\hbar}{2}
\begin{bmatrix}
  k_{\plus} \\
  k_{\minus}
\end{bmatrix}
\]
For $\frac{\hbar}{2}$, we get the
following equations:
\begin{align*}
  \frac{\hbar}{2}\cos\beta k_{\plus}
  +\frac{\hbar}{2}e^{-i\alpha}\sin\beta k_{\minus} &=
  \frac{\hbar}{2}k_{\plus} \\
  \frac{\hbar}{2}e^{i\alpha}\sin\beta k_{\plus}
  -\frac{\hbar}{2}\cos\beta k_{\minus} &=
  \frac{\hbar}{2}k_{\minus} \\
\end{align*}
We can factor out the $\frac{\hbar}{2}$ and move everything to the
left side to get
\begin{align*}
  e^{-i\alpha}\sin\beta k_{\minus} - (1 - \cos\beta)k_{\plus} &= 0 \\
  e^{i\alpha}\sin\beta k_{\plus} - (1 + \cos\beta)k_{\minus} &= 0 \\
\end{align*}
Combining these gives us
\begin{align*}
  e^{i\alpha}\sin\beta k_{\plus} + (1 - \cos\beta)k_{\plus} &=
  e^{-i\alpha}\sin\beta k_{\minus} + (1 + \cos\beta)k_{\minus} \\
  [e^{i\alpha}\sin\beta + (1 - \cos\beta)]k_{\plus} &=
  [e^{-i\alpha}\sin\beta + (1 + \cos\beta)]k_{\minus} \\
  \left[2e^{i\alpha}\cos\frac{\beta}{2}\sin\frac{\beta}{2} + 2\sin^2\frac{\beta}{2}\right]k_{\plus} &=
  \left[2e^{-i\alpha}\cos\frac{\beta}{2}\sin\frac{\beta}{2} + 2\cos^2\frac{\beta}{2}\right]k_{\minus} \\
  2\sin\frac{\beta}{2}\left[\sin\frac{\beta}{2} + e^{i\alpha}\cos\frac{\beta}{2}\right]k_{\plus} &=
  2e^{-i\alpha}\cos\frac{\beta}{2}\left[\sin\frac{\beta}{2} + e^{i\alpha}\cos^\frac{\beta}{2}\right]k_{\minus} \\
  e^{i\alpha}\sin\frac{\beta}{2}k_{\plus} &= \cos\frac{\beta}{2}k_{\minus} \\
  \frac{k_{\plus}}{\cos\frac{\beta}{2}} - \frac{k_{\minus}}{e^{i\alpha}\sin\frac{\beta}{2}} &= 0 \\
\end{align*}
This is solved by $k_{\plus} = \cos\frac{\beta}{2}, k_{\minus} =
e^{i\alpha}\sin\frac{\beta}{2}$, giving us the eigenket
\[ \cos\frac{\beta}{2}\ket{\plus} + e^{i\alpha}\sin\frac{\beta}{2}\ket{\minus} \]

For $-\frac{\hbar}{2}$ gives us the following equations:
\begin{align*}
  \frac{\hbar}{2}\cos\beta k_{\plus}
  +\frac{\hbar}{2}e^{-i\alpha}\sin\beta k_{\minus} &=
  -\frac{\hbar}{2}k_{\plus} \\
  \frac{\hbar}{2}e^{i\alpha}\sin\beta k_{\plus}
  -\frac{\hbar}{2}\cos\beta k_{\minus} &=
  -\frac{\hbar}{2}k_{\minus} \\
\end{align*}
The same procedure as before gives us
\begin{align*}
  e^{-i\alpha}\sin\beta k_{\minus} + (1 + \cos\beta)k_{\plus} &= 0 \\
  e^{i\alpha}\sin\beta k_{\plus} + (1 - \cos\beta)k_{\minus} &= 0 \\
\end{align*}
Combining these gives us
\begin{align*}
  e^{i\alpha}\sin\beta k_{\plus} - (1 + \cos\beta)k_{\plus} &=
  e^{-i\alpha}\sin\beta k_{\minus} - (1 - \cos\beta)k_{\minus} \\
  [e^{i\alpha}\sin\beta - (1 + \cos\beta)]k_{\plus} &=
  [e^{-i\alpha}\sin\beta - (1 - \cos\beta)]k_{\minus} \\
  \left[2e^{i\alpha}\cos\frac{\beta}{2}\sin\frac{\beta}{2} - 2\cos^2\frac{\beta}{2}\right]k_{\plus}
  &=
  \left[2e^{-i\alpha}\cos\frac{\beta}{2}\sin\frac{\beta}{2} - 2\sin^2\frac{\beta}{2}\right]k_{\minus} \\
  -2\cos\frac{\beta}{2}\left[\sin\frac{\beta}{2} - e^{i\alpha}\cos\frac{\beta}{2}\right]k_{\plus}
  &=
  2e^{-i\alpha}\sin\frac{\beta}{2}\left[\sin\frac{\beta}{2} - e^{i\alpha}\cos^\frac{\beta}{2}\right]k_{\minus} \\
  -e^{i\alpha}\cos\frac{\beta}{2}k_{\plus} &= \sin\frac{\beta}{2}k_{\minus} \\
  \frac{k_{\plus}}{\sin\frac{\beta}{2}} + \frac{k_{\minus}}{e^{i\alpha}\cos\frac{\beta}{2}} &= 0 \\
\end{align*}
This is solved by $k_{\plus} = \sin\frac{\beta}{2}, k_{\minus} =
-e^{i\alpha}\cos\frac{\beta}{2}$, giving us the eigenket
\[ \sin\frac{\beta}{2}\ket{\plus} - e^{i\alpha}\cos\frac{\beta}{2}\ket{\minus} \]
