Using the orthogonality of $\ket{\plus}$ and $\ket{\minus}$, prove
\begin{align*}
  [S_i,S_j] &= i\epsilon_{i,j,k}\hbar S_k \\
  \{S_i, S_j\} &= \left(\frac{\hbar^2}{2}\right)\delta_{ij}S_k
\end{align*}
where
\begin{align*}
  S_x
  &=
  \frac{\hbar}{2}(\outerprod{\plus}{\minus} + \outerprod{\minus}{\plus}) \\
  S_y
  &=
  \frac{i\hbar}{2}(\outerprod{\minus}{\plus} - \outerprod{\plus}{\minus}) \\
  S_z
  &=
  \frac{\hbar}{2}(\outerprod{\plus}{\plus} - \outerprod{\minus}{\minus})
\end{align*}

\subsection*{Solution}
Go ahead and derive the products
\begin{align*}
  S_{x}S_{x} &=
  \frac{\hbar}{2}(\outerprod{\plus}{\minus} + \outerprod{\minus}{\plus})
  \frac{\hbar}{2}(\outerprod{\plus}{\minus} + \outerprod{\minus}{\plus}) \\
  &=
  \left(\frac{\hbar}{2}\right)^2
  (\doubleouterprod{\plus}{\minus}{\plus}{\minus}
  +\doubleouterprod{\plus}{\minus}{\minus}{\plus}
  +\doubleouterprod{\minus}{\plus}{\plus}{\minus}
  +\doubleouterprod{\minus}{\plus}{\minus}{\plus}) \\
  &=
  \left(\frac{\hbar}{2}\right)^2
  (\outerprod{\plus}{\plus} + \outerprod{\minus}{\minus}) \\
  &=
  \left(\frac{\hbar}{2}\right)^2 I
\end{align*}
\begin{align*}
  S_{x}S_{y} &=
  \frac{\hbar}{2}(\outerprod{\plus}{\minus} + \outerprod{\minus}{\plus})
  \frac{i\hbar}{2}(\outerprod{\minus}{\plus} - \outerprod{\plus}{\minus}) \\
  &=
  i\left(\frac{\hbar}{2}\right)^2
  (\doubleouterprod{\plus}{\minus}{\minus}{\plus}
  -\doubleouterprod{\plus}{\minus}{\plus}{\minus}
  +\doubleouterprod{\minus}{\plus}{\minus}{\plus}
  -\doubleouterprod{\minus}{\plus}{\plus}{\minus}) \\
  &=
  i\left(\frac{\hbar}{2}\right)^2
  (\outerprod{\plus}{\plus} - \outerprod{\minus}{\minus}) \\
  &=
  \frac{i\hbar}{2}S_z
\end{align*}
\begin{align*}
  S_{x}S_{z} &=
  \frac{\hbar}{2}(\outerprod{\plus}{\minus} + \outerprod{\minus}{\plus})
  \frac{\hbar}{2}(\outerprod{\plus}{\plus} - \outerprod{\minus}{\minus}) \\
  &=
  \left(\frac{\hbar}{2}\right)^2
  (\doubleouterprod{\plus}{\minus}{\plus}{\plus}
  -\doubleouterprod{\plus}{\minus}{\minus}{\minus}
  +\doubleouterprod{\minus}{\plus}{\plus}{\plus}
  -\doubleouterprod{\minus}{\plus}{\minus}{\minus}) \\
  &=
  \left(\frac{\hbar}{2}\right)^2
  (\outerprod{\minus}{\plus} -\outerprod{\plus}{\minus}) \\
  &=
  -\frac{i\hbar}{2}S_y
\end{align*}
\begin{align*}
  S_{y}S_{x} &=
  \frac{i\hbar}{2}(\outerprod{\minus}{\plus} - \outerprod{\plus}{\minus})
  \frac{\hbar}{2}(\outerprod{\plus}{\minus} + \outerprod{\minus}{\plus}) \\
  &=
  i\left(\frac{\hbar}{2}\right)^2
  (\doubleouterprod{\minus}{\plus}{\plus}{\minus}
  -\doubleouterprod{\minus}{\plus}{\minus}{\plus}
  + \doubleouterprod{\plus}{\minus}{\plus}{\minus}
  - \doubleouterprod{\plus}{\minus}{\minus}{\plus}) \\
  &=
  i\left(\frac{\hbar}{2}\right)^2
  (\outerprod{\minus}{\minus} - \outerprod{\plus}{\plus}) \\
  &=
  -\frac{i\hbar}{2}S_z
\end{align*}
\begin{align*}
  S_{y}S_{y} &=
  \frac{i\hbar}{2}(\outerprod{\minus}{\plus} - \outerprod{\plus}{\minus})
  \frac{i\hbar}{2}(\outerprod{\minus}{\plus} - \outerprod{\plus}{\minus}) \\
  &=
  -\left(\frac{\hbar}{2}\right)^2
  (\doubleouterprod{\minus}{\plus}{\minus}{\plus}
  -\doubleouterprod{\minus}{\plus}{\plus}{\minus}
  - \doubleouterprod{\plus}{\minus}{\minus}{\plus}
  + \doubleouterprod{\plus}{\minus}{\plus}{\minus}) \\
  &=
  \left(\frac{\hbar}{2}\right)^2
  (\outerprod{\minus}{\minus} + \outerprod{\plus}{\plus}) \\
  &=
  \left(\frac{\hbar}{2}\right)^2 I
\end{align*}
\begin{align*}
  S_{y}S_{z} &=
  \frac{i\hbar}{2}(\outerprod{\minus}{\plus} - \outerprod{\plus}{\minus})
  \frac{\hbar}{2}(\outerprod{\plus}{\plus} - \outerprod{\minus}{\minus}) \\
  &=
  i\left(\frac{\hbar}{2}\right)^2
  (\doubleouterprod{\minus}{\plus}{\plus}{\plus}
  -\doubleouterprod{\minus}{\plus}{\minus}{\minus}
  - \doubleouterprod{\plus}{\minus}{\plus}{\plus}
  + \doubleouterprod{\plus}{\minus}{\minus}{\minus}) \\
  &=
  i\left(\frac{\hbar}{2}\right)^2
  (\outerprod{\minus}{\plus} + \outerprod{\plus}{\minus}) \\
  &=
  \frac{i\hbar}{2}S_x
\end{align*}
\begin{align*}
  S_{z}S_{x} &=
  \frac{\hbar}{2}(\outerprod{\plus}{\plus} - \outerprod{\minus}{\minus})
  \frac{\hbar}{2}(\outerprod{\plus}{\minus} + \outerprod{\minus}{\plus}) \\
  &=
  \left(\frac{\hbar}{2}\right)^2
  (\doubleouterprod{\plus}{\plus}{\plus}{\minus}
  -\doubleouterprod{\plus}{\plus}{\minus}{\plus}
  +\doubleouterprod{\minus}{\minus}{\plus}{\minus}
  -\doubleouterprod{\minus}{\minus}{\minus}{\plus}) \\
  &=
  \left(\frac{\hbar}{2}\right)^2
  (\outerprod{\plus}{\minus} -\outerprod{\minus}{\plus}) \\
  &=
  \frac{i\hbar}{2}S_y
\end{align*}
\begin{align*}
  S_{z}S_{y} &=
  \frac{\hbar}{2}(\outerprod{\plus}{\plus} - \outerprod{\minus}{\minus})
  \frac{i\hbar}{2}(\outerprod{\minus}{\plus} - \outerprod{\plus}{\minus}) \\
  &=
  i\left(\frac{\hbar}{2}\right)^2
  (\doubleouterprod{\plus}{\plus}{\minus}{\plus}
  -\doubleouterprod{\plus}{\plus}{\plus}{\minus}
  -\doubleouterprod{\minus}{\minus}{\minus}{\plus}
  +\doubleouterprod{\minus}{\minus}{\plus}{\minus}) \\
  &=
  -i\left(\frac{\hbar}{2}\right)^2
  (\outerprod{\plus}{\minus} + \outerprod{\minus}{\plus}) \\
  &=
  -\frac{i\hbar}{2}S_x
\end{align*}
\begin{align*}
  S_{z}S_{z} &=
  \frac{\hbar}{2}(\outerprod{\plus}{\plus} - \outerprod{\minus}{\minus})
  \frac{\hbar}{2}(\outerprod{\plus}{\plus} - \outerprod{\minus}{\minus}) \\
  &=
  \left(\frac{\hbar}{2}\right)^2
  (\doubleouterprod{\plus}{\plus}{\plus}{\plus}
  -\doubleouterprod{\plus}{\plus}{\minus}{\minus}
  -\doubleouterprod{\minus}{\minus}{\plus}{\plus}
  +\doubleouterprod{\minus}{\minus}{\minus}{\minus}) \\
  &=
  \left(\frac{\hbar}{2}\right)^2
  (\outerprod{\plus}{\plus} + \outerprod{\minus}{\minus}) \\
  &=
  \left(\frac{\hbar}{2}\right)^2 I
\end{align*}
First, it is immediate that $[S_i, S_i] = 0$.  Since all
\[
S_iS_i =
\left(\frac{\hbar}{2}\right)^2
(\outerprod{\plus}{\plus} + \outerprod{\minus}{\minus})
\]
we have
\begin{align*}
  \{S_i, S_i\} &= S_iS_i + S_iS_i \\
  &=
  2\left(\frac{\hbar}{2}\right)^2
  (\outerprod{\plus}{\plus} + \outerprod{\minus}{\minus}) \\
  &=
  \frac{\hbar^2}{2}I \\
\end{align*}
So the relation holds.

For the anticommutator, it is enough to examine the forward cycles
(since $\{ A, B \} = \{ A, B \}$).
\begin{align*}
  \{S_x, S_y\} &= S_xS_y + S_yS_x \\
  &=
  \frac{i\hbar}{2}S_z - \frac{i\hbar}{2}S_z \\
  &=
  0
\end{align*}
\begin{align*}
  \{S_y, S_z\} &= S_yS_z + S_zS_y \\
  &=
  \frac{i\hbar}{2}S_x - \frac{i\hbar}{2}S_x \\
  &=
  0
\end{align*}
\begin{align*}
  \{S_z, S_x\} &= S_zS_x + S_xS_z \\
  &=
  \frac{i\hbar}{2}S_y - \frac{i\hbar}{2}S_y \\
  &=
  0
\end{align*}
Now examine the forward cycles for the commutator.
\begin{align*}
  [S_x, S_y] &= S_xS_y - S_yS_x \\
  &=
  \frac{i\hbar}{2}S_z + \frac{i\hbar}{2}S_z \\
  &= i\hbar S_z
\end{align*}
\begin{align*}
  [S_y, S_z] &= S_yS_z - S_zS_y \\
  &=
  \frac{i\hbar}{2}S_x + \frac{i\hbar}{2}S_x \\
  &=
  i\hbar S_x
\end{align*}
\begin{align*}
  [S_z, S_x] &= S_zS_x - S_xS_z \\
  &=
  \frac{i\hbar}{2}S_y + \frac{i\hbar}{2}S_y \\
  &=
  i\hbar S_y
\end{align*}

For the reverse cycles, use the identity $[A, B] = -[B, A]$ to obtain
the expected values.
