Prove the following:
\[ [AB, CD] = -AC\{D,B\} + A\{C,B\}D - C\{D, A\}B + \{C,A\}DB \]

\subsection*{Solution}
Rewrite as follows:
\begin{align*}
 [AB, CD] &= -AC\{D, B\} + A\{C, B\}D - C\{D, A\}B + \{C,A\}DB \\
 &= -AC(DB + BD) + A(CB + BC)D - C(DA + AD)B + (CA + AC)DB \\
 &= -ACDB - ACBD + ACBD + ABCD - CDAB - CADB + CADB + ACDB \\
 &= ACDB - ACDB + ACBD - ACBD + CADB - CADB + ABCD - CDAB  \\
 &= (ACDB - ACDB) + (ACBD - ACBD) + (CADB - CADB) + ABCD - CDAB \\
 &= ABCD - CDAB \\
 &= [AB, CD]
\end{align*}
